examples/unit-tests/rec.fst
@@ -16,33 +16,80 @@
 module Foo.Record
 
 
-let foo x y = 
-  if x <= y && y <= x 
-  then 0 
-  else 1
+let rec foo f = foo (fun x -> f x)
+
+let rec visit_pat0 k0 = k0 0
+and visit_pats0 k1 = visit_pat0 (fun _ -> visit_pats0 k1)
+  
+let rec visit_pat1 pat cont = cont (0, pat)
+and visit_pats1 pat cont = visit_pat1 pat (fun (_,_) -> visit_pats1 pat (fun z -> cont 0))
+
+(* let rec visit_pat1 pat cont = cont (0, pat) *)
+(* and visit_pats1 pats cont = match pats with *)
+(*   | hd::tl -> visit_pat1 hd (fun (_, hd) -> *)
+(*     visit_pats1 tl (fun _ -> *)
+(*       cont (hd::tl))) *)
+
+let rec visit_pat2 env pat cont = cont (env, pat)
+and visit_pats2 env pats cont = match pats with
+  | hd::tl -> visit_pat2 env  hd (fun (env, hd) ->
+    visit_pats2 env tl (fun (env, tl) ->
+      cont (env, hd::tl)))
 
 type r = {
-  a:int; 
+  a:int;
   b:int;
 }
+let withb b a = {a=a; b=b}
+let zr r =
+  let w = withb r.b in
+  w 0
 
-let matchr r = match r with 
-  | ({a=_}) -> 1
+let rec ff x = let y = 0 in ff y
 
-type pair = {x:int; y:int}
-and triple = {fst:pair; z:int}
+let rec cps_len x k = match x with
+  | [] -> k 0
+  | hd::tl -> cps_aux hd (fun n -> cps_len tl (fun i -> k (i + n)))
+and cps_aux x k = match x with
+  | [] -> k 0
+  | hd::tl -> cps_aux tl (fun n -> k (n + 1))
 
-let mkR i j = {a=i; b=j}
-let mkPair i j = {x=i; y=j}
-let mkFoo i = {fst={x=i; y=i}; z=i}
+type t =
+  | Leaf of int
+  | Node of list t
 
-let a x = x.a
-let f x y = {x=x; y=y}
-let g p = p.x
-let h p = p.y
-let i p = match p with
-  | {fst=_} -> ""
+let rec vt x f k = match x with
+  | Leaf i -> k (f i)
+  | Node xs -> vts xs f k
+and vts xs f k = match xs with
+  | [] -> k 0
+  | hd::tl -> vt hd f (fun l -> vts tl f (fun m -> k (l+m)))
 
-let rec even x = x=0 || not (odd (x - 1))
-and odd x = x=1 || not (even (x - 1))
+
+ 
+(* let foo x y = *)
+(*   if x <= y && y <= x *)
+(*   then 0 *)
+(*   else 1 *)
+
+
+(* let matchr r = match r with *)
+(*   | ({a=_}) -> 1 *)
+
+(* type pair = {x:int; y:int} *)
+(* and triple = {fst:pair; z:int} *)
+
+(* let mkR i j = {a=i; b=j} *)
+(* let mkPair i j = {x=i; y=j} *)
+(* let mkFoo i = {fst={x=i; y=i}; z=i} *)
+
+(* let a x = x.a *)
+(* let f x y = {x=x; y=y} *)
+(* let g p = p.x *)
+(* let h p = p.y *)
+(* let i p = match p with *)
+(*   | {fst=_} -> "" *)
+(* 1 *)
+(* let rec even x = x=0 || not (odd (x - 1)) *)
+(* and odd x = x=1 || not (even (x - 1)) *)
 
